

$x_1 = 1$	$y_1 = 1$
$x_2 = 3$	$y_2 = -1$

Find the output value of $z=2$

- Use polynomial kernel

$$K(x, y) = (x^T y + 1)^d$$

- set kernel parameter, $d=1$ (degree 1)

$$K(x, y) = (xy + 1) \Rightarrow K(x_i, x_j) = (x_i x_j + 1)$$

- C is set to 5

- Value of α_i determination where $i = 1$ to 2
 $j = 1$ to 2

$$\max \left[\sum_{i=1}^2 \alpha_i - \frac{1}{2} \sum_{i=1}^2 \sum_{j=1}^2 \alpha_i \alpha_j y_i y_j (x_i x_j + 1) \right]$$

subject to the constraints

$$5 \gg \alpha_i \gg 0 \quad \text{and} \quad \sum_{i=1}^2 \alpha_i y_i = 0$$

$$\text{Here, } \max \left[\sum_{i=1}^2 \alpha_i - \frac{1}{2} \sum_{i=1}^2 \sum_{j=1}^2 \alpha_i \alpha_j y_i y_j (x_i x_j + 1) \right]$$

$$= \max \left[(\alpha_1 + \alpha_2) - \frac{1}{2} \left[\alpha_1 \alpha_1 y_1 y_1 (x_1 x_1 + 1) + \alpha_1 \alpha_2 y_1 y_2 (x_1 x_2 + 1) + \alpha_2 \alpha_1 y_2 y_1 (x_2 x_1 + 1) + \alpha_2 \alpha_2 y_2 y_2 (x_2 x_2 + 1) \right] \right]$$

$$\left[\text{Put } x_1 = 1, x_2 = 3 \right. \\ \left. y_1 = 1, y_2 = -1 \right]$$

$$= \max \left[-\alpha_1^2 + 5\alpha_1\alpha_2 - 5\alpha_2^2 \right]$$

$$\text{subject to } \sum_{i=1}^2 \alpha_i y_i = 0$$

$$\Rightarrow \alpha_1 y_1 + \alpha_2 y_2 = 0$$

$$\Rightarrow \alpha_1 \cdot 1 + \alpha_2 \cdot (-1) = 0$$

$$\Rightarrow \alpha_1 - \alpha_2 = 0$$

$$\text{and } 0 \leq \alpha_i \leq c$$

$$\Rightarrow 0 \leq \alpha_i \leq 5$$

$$\therefore \text{maximize } -\alpha_1^2 + 5\alpha_1\alpha_2 - 5\alpha_2^2$$

$$\text{subject to } \alpha_1 - \alpha_2 = 0$$

$$\text{and } 0 \leq \alpha_i \leq 5$$

$$\text{Let, } f(\alpha_1, \alpha_2) = -\alpha_1^2 + 5\alpha_1\alpha_2 - 5\alpha_2^2$$

$$g(\alpha_1, \alpha_2) = \alpha_1 - \alpha_2$$

Assume, Lagrange's multiplier, λ [$\lambda \neq 0$]

$$\frac{\partial f}{\partial \alpha_1} + \lambda \frac{\partial g}{\partial \alpha_1} = 0$$

$$\frac{\partial f}{\partial \alpha_2} + \lambda \frac{\partial g}{\partial \alpha_2} = 0$$

$$\frac{\partial f}{\partial \alpha_1} = \frac{\partial}{\partial \alpha_1} (-\alpha_1^2 + 5\alpha_1 \alpha_2 - 5\alpha_2^2) = -2\alpha_1 + 5\alpha_2$$

$$\frac{\partial g}{\partial \alpha_1} = \frac{\partial}{\partial \alpha_1} (\alpha_1 - \alpha_2) = 1$$

Again,

$$\frac{\partial f}{\partial \alpha_2} = \frac{\partial}{\partial \alpha_2} (-\alpha_1^2 + 5\alpha_1 \alpha_2 - 5\alpha_2^2) = 5\alpha_1 - 10\alpha_2$$

$$\frac{\partial g}{\partial \alpha_2} = \frac{\partial}{\partial \alpha_2} (\alpha_1 - \alpha_2) = -1$$

$$\frac{\partial f}{\partial \alpha_1} + \lambda \frac{\partial g}{\partial \alpha_1} = 0$$

$$\Rightarrow -2\alpha_1 + 5\alpha_2 + \lambda \cdot 1 = 0$$

$$\Rightarrow 2\alpha_1 - 5\alpha_2 - \lambda = 0 \quad \dots \text{eq ①}$$

$$\frac{\partial f}{\partial \alpha_2} + \lambda \frac{\partial g}{\partial \alpha_2} = 0$$

$$\Rightarrow 5\alpha_1 - 10\alpha_2 + \lambda \cdot (-1) = 0$$

$$\Rightarrow 5\alpha_1 - 10\alpha_2 - \lambda = 0$$

$$\dots \text{eq ②}$$

$$\text{eq ②} - \text{eq ①} \Rightarrow$$

$$3\alpha_1 - 5\alpha_2 = 0$$

$$\Rightarrow \alpha_1 = -\frac{5}{3}\alpha_2$$

$$\text{from eq ①} \Rightarrow$$

$$2\alpha_1 - 5\alpha_2 - \lambda = 0$$

$$\Rightarrow \cancel{2\alpha_1} - 2 \cdot \frac{5}{3}\alpha_2 - 5\alpha_2 - \lambda = 0$$

$$\Rightarrow -\frac{5}{3}\alpha_2 - \lambda = 0$$

$$\Rightarrow \alpha_2 = -\frac{3}{5}\lambda$$

$$\therefore \alpha_1 = \frac{5}{3} * \left(-\frac{3}{5}\lambda\right) = -\lambda$$

$$\therefore \alpha_1 = -\lambda$$

$$\alpha_2 = -\frac{3}{5}\lambda$$

$$\text{if } \lambda = -c \\ = -5,$$

$$\alpha_1 = -(-5) = 5$$

$$\alpha_2 = -\frac{3}{5}\lambda \\ = -\frac{3}{5}(-5)$$

$$= 3$$

$$\text{since } \alpha_1 - \alpha_2 = 0 \\ \Rightarrow \alpha_2 = 5$$

$$\text{since } \alpha_1 - \alpha_2 = 0 \\ \Rightarrow \alpha_2 = 3$$

$$\alpha_1 = 5, 3 \\ \alpha_2 = 5, 3$$

solution

Additional

Again

from eq (ii) \Rightarrow

$$5\alpha_1 - 10\alpha_2 - \lambda = 0$$

$$\Rightarrow 5 \cdot \frac{5}{3}\alpha_2 - 10\alpha_2 - \lambda = 0$$

$$\Rightarrow \frac{25}{3}\alpha_2 - 10\alpha_2 - \lambda = 0$$

$$\Rightarrow -\frac{5}{3}\alpha_2 - \lambda = 0$$

$$\Rightarrow \alpha_2 = -\frac{3}{5}\lambda$$

$$\text{where } \alpha_1 = \frac{5}{3}\alpha_2$$

$$\text{for } \lambda = -c, \alpha_1 = -\lambda = c = 5$$

$$\alpha_2 = -\frac{3}{5}\lambda = -\frac{3}{5}(-5) \\ = 3$$

$$= \frac{5}{3} * \left(-\frac{3}{5}\lambda\right) \\ = -\lambda$$

$$\alpha_1 = 5 \\ \alpha_2 = 3$$

solution

data, $z=2$,

Page = 5

$$\begin{aligned} f(z) &= -4z + 5 \\ \Rightarrow f(2) &= -4 \times 2 + 5 \\ &= -8 + 5 \end{aligned}$$

$$= -3$$

\Rightarrow Negative class

\therefore for, $z=2$, output class = -1

$$f(d_1, d_2) =$$

$$f(d_1, d_2) = d_1^2 + 5d_1d_2 - 5d_2^2$$

$$= -d_1^2 + 5d_1^2 - 5d_1^2 \quad [d_1 = d_2]$$

$$= -d_1^2$$

$$= -5^2$$

$$[d_1 = 5]$$

$$= -25$$

$$\underline{\underline{-25}} \quad f(d_1, d_2)$$

$$\text{Again, } = -d_1^2 + 5d_1d_2 - 5d_2^2$$

$$= -d_1^2$$

$$= -9$$

$$[d_1 = 3]$$

Here, maximum value is -9 for $d_1 = 3$

$$\text{So, } \underline{\underline{d_1 = 3}}, \quad \underline{\underline{d_2 = 3}}$$

$$\boxed{\begin{array}{l} d_1 = 3 \\ d_2 = 3 \end{array}}$$

Testing

Page 6

$$\begin{array}{lll} x_1 = 1 & y_1 = 1 & \alpha_1 = 3 \\ x_2 = 3 & y_2 = -1 & \alpha_2 = 3 \end{array}$$

Discriminant function,

$$f(z) = \sum_{j=1}^s \alpha_{t_j} y_{t_j} \kappa(x_{t_j}, z) + b$$

$$= \sum_{j=1}^2 \alpha_{t_j} y_{t_j} \kappa(x_{t_j}, z) + b$$

$$= \alpha_1 y_1 (x_1 z + 1) + \alpha_2 y_2 (x_2 z + 1) + b$$

$$= 3 * 1 (1 \cdot z + 1) + 3 * (-1) (3z + 1) + b$$

$$= 3z + 3 - 9z - 3 + b$$

$$= -6z + b$$

if $z = x_1 = 1$

$$f(x_1) = -6x_1 + b$$

$$\Rightarrow y_1 = -6 * 1 + b$$

$$\Rightarrow 1 = -6 + b$$

$$\Rightarrow b = 7$$

* Discriminant function, $f(z) = -6z + 7$

* New data, $z = 2$, $f(z) = -6z + 7$

$$= -6 * 2 + 7$$

$$= -12 + 7$$

$$= -5 = \text{Negative class}$$

For test data 2, output class = -1